theories/caesium/notation.v
@@ -66,6 +66,15 @@ Notation "e1 <<c{ ot1 , ot2 } e2" := (CheckBinOp ShlOp ot1 ot2 e1%E e2%E)
 Notation "e1 >>c{ ot1 , ot2 } e2" := (CheckBinOp ShrOp ot1 ot2 e1%E e2%E)
   (at level 70, format "e1  >>c{ ot1 ,  ot2 }  e2") : expr_scope.
 
+(* Unchecked operations *)
+Notation "e1 '+unchecked' '{' ot1 , ot2 } e2" := (BinOp UncheckedAddOp ot1 ot2 e1%E e2%E)
+  (at level 50, left associativity, format "e1  '+unchecked' '{' ot1 ,  ot2 }  e2") : expr_scope.
+Notation "e1 '-unchecked' '{' ot1 , ot2 } e2" := (BinOp UncheckedSubOp ot1 ot2 e1%E e2%E)
+  (at level 50, left associativity, format "e1  '-unchecked' '{' ot1 ,  ot2 }  e2") : expr_scope.
+Notation "e1 ×unchecked{ ot1 , ot2 } e2" := (BinOp UncheckedMulOp ot1 ot2 e1%E e2%E)
+  (at level 70, format "e1  ×unchecked{ ot1 ,  ot2 }  e2") : expr_scope.
+
+
 (* The offset must be evaluated first for the type system to work, thus the order is switched here. *)
 Notation "e1 'at_offset{' ly , ot1 , ot2 } e2" := (BinOp (PtrOffsetOp ly) ot2 ot1 e2%E e1%E)
   (at level 70, format "e1  at_offset{ ly ,  ot1 ,  ot2 }  e2") : expr_scope.
